Examples.v
@@ -1,8 +1,20 @@
 From vchez Require Export Definitions.
 From vchez Require Export Pass.
+From vchez Require Export Semantics.
 From vchez Require Import Helpers.
+
 From Coq Require Import List.
 Import ListNotations.
+
+(* reworking examples with new syntax 
+(*Semantics examples*)
+
+Example sem1 : forall sfs,
+  multi_step sfs (s_trm_car (s_trm_cons s_trm_true s_trm_false))
+             sfs (s_trm_true).
+Proof.
+  intros. repeat constructor.
+
 
 (* Examples of the convert-assignments pass working as intended *)
 
@@ -31,3 +43,4 @@ Example ca_6 :
           t_trm_false).
 Proof. reflexivity. Qed.
 
+*)
