Framework.v
@@ -3,8 +3,8 @@ From TLC Require Import LibLN.
 From TLC Require Import LibReflect.
 From Coq Require Export List.
 
-Hint Constructors s_term : core.
-Hint Constructors t_term : core.
+Hint Constructors s_trm.
+Hint Constructors s_term.
 
 (* Properties of local closure *)
 Lemma s_term_abs_to_body : forall ts,
@@ -12,39 +12,17 @@ Lemma s_term_abs_to_body : forall ts,
 Proof.
   intros. unfold s_body. inversion* H. Qed.
 
-Lemma t_term_abs_to_body : forall ts,
-  t_term (t_trm_abs ts) -> t_body ts.
-Proof.
-  intros. unfold t_body. inversion* H. Qed.
-
 Lemma s_body_to_term_abs : forall ts,
   s_body ts -> s_term (s_trm_abs ts).
 Proof.
   intros. inversion* H. Qed.
 
-Lemma t_body_to_term_abs : forall ts,
-  t_body ts -> t_term (t_trm_abs ts).
-Proof.
-  intros. inversion* H. Qed.
-
-Hint Resolve s_term_abs_to_body 
-             t_term_abs_to_body 
-             s_body_to_term_abs
-             t_body_to_term_abs.
+Hint Resolve s_term_abs_to_body  
+             s_body_to_term_abs.
 
 Lemma s_subst_id : forall t x u,
   x \notin s_fv t -> s_subst x u t = t.
-Proof.
-  intros. induction t; simpls; f_equal~; eauto.
-  induction ts; simpls. reflexivity.
-  - apply notin_union in H. destruct H. rewrite IHts.
-    + f_equal~. admit.
-    + apply H0.
-  - admit.
-  - unfold notin in H. rewrite in_singleton in H.   
-    + rewrite var_compare_eq. rewrite if_isTrue.
-      unfold not in H. admit.
-Admitted.
+Proof. Abort. 
 
 
      
